Define weakest precondition for threadpools in preparation for porting threadpool adequacy to new definition of `WPi`.

src/threadpool.v
@@ -2,9 +2,11 @@ From iris.proofmode Require Import proofmode.
 From iris.base_logic.lib Require Import iprop.
 From iris.base_logic.lib Require Import ghost_var.
 From iris.base_logic.lib Require Export fancy_updates.
+From iris.bi Require Import fixpoint.
 From iris.itree Require Import handler.
 From iris.itree Require Import wpi.
 From iris.itree Require Import itree.
+From iris.itree Require Import axioms.
 From ITree Require Import ITree.
 From ITree Require Import Eq.
 From stdpp Require Import list.
@@ -28,7 +30,7 @@ Variant threadpoolE : Type → Type :=
   | EKillThread : threadpoolE Empty_set.
 
 (** [iHandler] for [threadpoolE]. *)
-Program Definition threadpoolH {Σ} `{!invGS_gen HasNoLc Σ} : iHandler Σ threadpoolE :=
+Program Definition threadpoolH {Σ} `{!invGS_gen hlc Σ} : iHandler Σ threadpoolE :=
   IHandler (λ A e,
     match e with
     (** We define the iHandler in a way that imposes a semantic restriction on
@@ -42,7 +44,7 @@ Program Definition threadpoolH {Σ} `{!invGS_gen HasNoLc Σ} : iHandler Σ threa
     end
   )%I _.
 Next Obligation.
-  iIntros (????????) "HΦwand #Hswand". destruct e.
+  iIntros (?????????) "HΦwand #Hswand". destruct e.
   - iIntros "[HΦ Hs]". iSplitL "HΦwand HΦ".
     * by iApply "HΦwand".
     * by iApply "Hswand".
@@ -51,18 +53,18 @@ Next Obligation.
 Qed.
 
 Section wp_threadpool.
-  Context `{!invGS_gen HasNoLc Σ} {E : Type → Type} {H : iHandler Σ E}.
+  Context `{!invGS_gen hlc Σ} {E : Type → Type} {H : iHandler Σ E}.
   Context `{threadpoolE -< E} `{inH Σ threadpoolE E threadpoolH H}.
 
   Lemma wpi_fork {R} (k : thread → itree E R) (M : coPset) (Φ : R → iProp Σ) :
-    (▷ WPi (k CurrentThread) @ H; M {{ Φ }} ∗ ▷ WPi (k NewThread) @ H; ⊤ {{ _, False }}) -∗
+    WPi (k CurrentThread) @ H; M {{ Φ }} ∗ WPi (k NewThread) @ H; ⊤ {{ _, False }} -∗
     WPi (vis EFork k) @ H; M {{ Φ }}.
   Proof.
     iIntros "[Hwpcur Hwpnew]". iApply wpi_vis.
     rewrite /threadpoolH. iFrame.
     iApply fupd_mask_intro; first apply empty_subseteq. iIntros "Hfupd".
     iApply is_inH. simpl. iSplitL "Hwpcur Hfupd".
-    - iNext. iMod "Hfupd". by iApply wpi_update_post_emp_mask.
+    - rewrite -wpi_clear_mask. iApply wpi_update. iMod "Hfupd". iMod "Hwpcur". by iModIntro.
     - done.
   Qed.
 
@@ -71,13 +73,13 @@ Section wp_threadpool.
   invariants. It amounts to the typical requirement of atomicity in the
   invariant opening rule known from "normal Iris". *)
   Lemma wpi_yield {R} (k : unit → itree E R) (M : coPset) (Φ : R → iProp Σ) :
-    (▷ WPi (k tt) @ H; ⊤ {{ Φ }}) -∗
+    WPi (k tt) @ H; ⊤ {{ Φ }} -∗
     WPi (vis EYield k) @ H; ⊤ {{ Φ }}.
   Proof.
     iIntros "Hwp". iApply wpi_vis. iApply is_inH. simpl.
     iApply fupd_mask_intro_subseteq; first done.
     iApply fupd_mask_intro; first apply empty_subseteq. iIntros "Hfupd".
-    iNext. rewrite -wpi_clear_mask. iMod "Hfupd". by iMod "Hwp".
+    rewrite -wpi_clear_mask. iApply wpi_update. iMod "Hfupd". by iMod "Hwp".
   Qed.
 
   Lemma wpi_kill {R} (k : Empty_set → itree E R) (M : coPset) (Φ : R → iProp Σ) :
@@ -88,18 +90,8 @@ Section wp_threadpool.
   Qed.
 End wp_threadpool.
 
-Lemma big_sepL_delete' {Σ} A (Φ : A → iProp Σ) l i x :
-  l !! i = Some x →
-  ([∗ list] y ∈ l, Φ y) ⊣⊢
-  Φ x ∗ [∗ list] y ∈ (delete i l), Φ y.
-Proof.
-  intros Hidx. rewrite -(take_drop_middle l i x) // !big_sepL_app.
-  rewrite assoc -!(comm _ (Φ _)) -assoc -big_sepL_app. do 2 f_equiv.
-  rewrite -delete_take_drop. f_equiv. rewrite take_drop_middle //.
-Qed.
-
 Section interleaving.
-  Context `{!invGS_gen HasNoLc Σ} {E : Type → Type} {H : iHandler Σ E} {R : Type}.
+  Context `{!invGS_gen hlc Σ} {E : Type → Type} {H : iHandler Σ E} {R : Type}.
   (** This sequentiality assumption is used for the [Emit] case in the adequacy
   proof below. *)
   Context `{!Sequential H}.
@@ -178,7 +170,419 @@ Section interleaving.
   Definition interleaves :
     list (itree (threadpoolE +' E) R) → itree (threadpoolE +' E) R → itree E R → Prop :=
     paco3 interleaves_ bot3.
+End interleaving.
 
+(* To prove adequacy for the threadpool handler, we need an induction principle
+for an entire threadpool as opposed to for a weakest precondition of a
+single thread. Therefore, it is necessary to define a weakest precondition for
+threadpools. However, this is only a necessity for the proof. It does not
+affect the statement of adequacy. *)
+Section wptp.
+  Context {Σ : gFunctors} {R : Type} {E : Type → Type} `{!invGS_gen hlc Σ}.
+
+  (** An intermediate definition to placate Coq's dependent pattern matching mechanism. *)
+  Definition handle_threadpoolE
+    (t : itree (threadpoolE +' E) R)
+    (tp : list (itree (threadpoolE +' E) R))
+    (Φ : leibnizO R -> iPropO Σ)
+    (wptp : leibnizO (itree (threadpoolE +' E) R) -> leibnizO (list (itree (threadpoolE +' E) R)) -> (leibnizO R -> iPropO Σ) -> iPropO Σ)
+    (A : Type)
+    (e : threadpoolE A)
+    : (A → itree (threadpoolE +' E) R) → iProp Σ :=
+    (** Trick: To have Coq not complain about dependent types, it is important
+    to introduce the dependently typed binders sufficiently late. This is why
+    we put a lambda after each arm, as opposed to on the outside. *)
+    match e with
+    | EKillThread => λ k,
+      |={∅, ⊤}=> |={⊤, ∅}=>
+      ( ∀ new_current_tid new_current,
+        ⌜tp !! new_current_tid = Some new_current⌝ →
+        wptp new_current (delete new_current_tid tp) Φ
+      )
+    | EYield => λ k,
+      |={∅, ⊤}=> |={⊤, ∅}=>
+      ( ∀ new_current_tid new_current,
+          ⌜tp !! new_current_tid = Some new_current⌝ →
+          wptp new_current (cons (Tau (k tt)) (delete new_current_tid tp)) Φ
+      ∨ wptp (k tt) tp Φ
+      )
+    | EFork => λ k,
+      wptp (k CurrentThread) (cons (k NewThread) tp) Φ
+    end%I.
+  (** The definition of the weakest precondition, prior to taking the fixpoint. *)
+  (* TODO: Uncurry this, and don't use the -n> to iProp *)
+  Definition wptpF (H : iHandler Σ E)
+    (wptp : leibnizO (itree (threadpoolE +' E) R) -> leibnizO (list (itree (threadpoolE +' E) R)) -> (R -d> iPropO Σ) -> iPropO Σ) :
+            leibnizO (itree (threadpoolE +' E) R) -> leibnizO (list (itree (threadpoolE +' E) R)) -> (R -d> iPropO Σ) -> iPropO Σ :=
+    λ t tp Φ,
+      (|={∅}=>
+        match observe t with
+        | RetF r  => |={∅, ⊤}=> Φ r
+        | TauF t' => wptp t' tp Φ
+        | @VisF _ _ _  A (inl1 e) k => handle_threadpoolE t tp Φ wptp A e k
+        | VisF (inr1 e) k => H _ e
+            (λ a, wptp (k a) tp Φ)
+            (λ a, |={⊤, ∅}=> wptp (k a) tp (λ _, False))
+        end
+      )%I.
+  Definition wptpF' (H : iHandler Σ E)
+    (wptp : leibnizO (itree (threadpoolE +' E) R) * leibnizO (list (itree (threadpoolE +' E) R)) * (R -d> iPropO Σ) -> iPropO Σ) :
+            leibnizO (itree (threadpoolE +' E) R) * leibnizO (list (itree (threadpoolE +' E) R)) * (R -d> iPropO Σ) -> iPropO Σ :=
+    λ pair, match pair with (t, tp, Φ) => wptpF H (curry3 wptp) t tp Φ end.
+
+  Global Instance wptpF_ne n H :
+    Proper ((dist n ==> dist n) ==> dist n ==> dist n) (wptpF' H).
+  Proof.
+    intros wp1 wp2 Hwp [[t1 tp1] Q1] [[t2 tp2] Q2] [[Ht Htp] HQ]. simpl in Ht, Htp, HQ.
+    rewrite /wptpF'/wptpF. destruct Ht, Htp. do 2 f_equiv. do 2 f_equiv.
+    - rewrite /curry3. by apply Hwp.
+    - destruct e as [e'|e'].
+      * rewrite /handle_threadpoolE. destruct e'.
+        + by apply Hwp.
+        + repeat f_equiv; eauto.
+        + do 3 f_equiv. intros new_current_tid. f_equiv. intros new_current. f_equiv.
+          rewrite /curry3. by apply Hwp.
+      * apply handler_ne.
+        + intros a. by apply Hwp.
+        + intros a. f_equiv. by apply Hwp.
+  Qed.
+
+  Lemma wptpF_mono H wptp1 wptp2:
+    ⊢ □ (∀ t tp Φ, wptp1 t tp Φ -∗ wptp2 t tp Φ)
+    → ∀ t tp Φ, wptpF H wptp1 t tp Φ -∗ wptpF H wptp2 t tp Φ.
+  Proof.
+    iIntros "#Hwand" (t tp Φ) "Hwp". rewrite /wptpF. destruct (observe t).
+    - done.
+    - by iApply "Hwand".
+    - rewrite /handle_threadpoolE. destruct e as [e|e].
+      * destruct e.
+        + by iApply "Hwand".
+        + iModIntro. iMod "Hwp". iMod "Hwp". iModIntro. iMod "Hwp". iModIntro.
+          iIntros (new_current_tid new_current Hidx).
+          iDestruct ("Hwp" $! new_current_tid new_current Hidx) as "[Hwp|Hwp]".
+          ++ iLeft. by iApply "Hwand".
+          ++ iRight. by iApply "Hwand".
+        + iMod "Hwp". iModIntro. iMod "Hwp". iModIntro. iMod "Hwp". iModIntro.
+          iIntros (new_current_tid new_current Hidx). iApply "Hwand". by iApply "Hwp".
+      * iMod "Hwp". iModIntro. iApply ihandler_mono.
+        + eauto.
+        + eauto.
+        + iApply ihandler_mono; last done.
+          ++ iIntros (a) "Hwp". by iApply "Hwand".
+          ++ iModIntro. iIntros (a) "Hwp". iMod "Hwp". iModIntro. by iApply "Hwand".
+  Qed.
+  Lemma wptpF_mono' H wp1 wp2:
+    ⊢ □ (∀ t tp Φ, wp1 (t, tp, Φ) -∗ wp2 (t, tp, Φ))
+    → ∀ t tp Φ, wptpF' H wp1 (t, tp, Φ) -∗ wptpF' H wp2 (t, tp, Φ).
+  Proof.
+    iApply wptpF_mono.
+  Qed.
+
+  Global Instance wp_itree_pre_monotone H :
+    BiMonoPred (λ wp_itree, wptpF' H wp_itree).
+  Proof.
+    constructor.
+    - iIntros (Π Ψ ??) "#Hinner". iIntros ([[??]?]) "Hsim" => /=. iApply wptpF_mono'; [|done].
+      iModIntro. iIntros (t tp Φ) "HΠ". by iApply "Hinner".
+    - intros wpi HneΦ n [t Φ] [t' Φ'] [-> HΦ]. f_equiv. simpl. by f_equiv.
+  Qed.
+
+  (* TODO: Rename [wpi] to [wpi_no_mask] or something along those lines. *)
+  Definition wptp (H : iHandler Σ E) (t : itree (threadpoolE +' E) R) (tp : list (itree (threadpoolE +' E) R)) (Φ : R -> iPropO Σ) : iProp Σ :=
+    bi_least_fixpoint (wptpF' H) ((t, tp), Φ).
+
+  Lemma wptp_unfold H t tp Φ :
+    wptp H t tp Φ ⊣⊢ wptpF H (wptp H) t tp Φ.
+  Proof.
+    apply: least_fixpoint_unfold.
+  Qed.
+End wptp.
+
+Section wptp_induction.
+  Context {Σ : gFunctors} {R : Type} {E : Type → Type} `{!invGS_gen hlc Σ} {H : iHandler Σ E}.
+
+  Lemma wptp_ind (G : leibnizO (itree (threadpoolE +' E) R) -> leibnizO (list (itree (threadpoolE +' E) R)) -> (R -d> iPropO Σ) -> iPropO Σ):
+    NonExpansive3 G →
+    (□ ∀ t tp Φ, wptpF H (λ t' tp' Ψ, G t' tp' Ψ ∧ wptp H t' tp' Ψ) t tp Φ -∗ G t tp Φ) -∗
+    ∀ t tp Φ, wptp H t tp Φ -∗ G t tp Φ.
+  Proof.
+    iIntros (Hne) "#HPre". iIntros (t tp Φ) "Hwptp".
+    rewrite {2}/wptp.
+    unshelve iApply (least_fixpoint_ind _ (uncurry3 G) with "[] Hwptp").
+    iIntros "!>" ([[??]?]) "Hwp" => /=. by iApply "HPre".
+  Qed.
+
+  Lemma wptp_iter (G : leibnizO (itree (threadpoolE +' E) R) -> leibnizO (list (itree (threadpoolE +' E) R)) -> (R -d> iPropO Σ) -> iPropO Σ) :
+    NonExpansive3 G →
+    (□ ∀ t tp Φ, wptpF H G t tp Φ -∗ G t tp Φ) -∗
+    ∀ t tp Φ, wptp H t tp Φ -∗ G t tp Φ.
+  Proof.
+    iIntros (Hne) "#HPre". iApply wptp_ind. iIntros "!>" (t tp Φ) "Hwptp".
+    iApply "HPre". iApply (wptpF_mono with "[] Hwptp").
+    iIntros "!>" (???) "[? _]". by iFrame.
+  Qed.
+
+  Lemma wptp_iter' (G : leibnizO (itree (threadpoolE +' E) R) -> leibnizO (list (itree (threadpoolE +' E) R)) -> (R -d> iPropO Σ) -> iPropO Σ):
+    NonExpansive3 G →
+    (□ ∀ Φ tp r, (|={∅,⊤}=> Φ r) -∗ G (Ret r) tp Φ) -∗
+    (□ ∀ Φ tp t, (|={∅}=> G t tp Φ) -∗ G (Tau t) tp Φ) -∗
+    (□ ∀ Φ tp k,
+      (|={∅, ⊤}=> |={⊤, ∅}=> ∀ new_current_tid new_current,
+        ⌜tp !! new_current_tid = Some new_current⌝ →
+        G new_current (delete new_current_tid tp) Φ) -∗
+      G (Vis (inl1 EKillThread) k) tp Φ
+    ) -∗
+    (□ ∀ Φ k tp,
+      (|={∅, ⊤}=> |={⊤, ∅}=>
+        (∀ new_current_tid new_current,
+            ⌜tp !! new_current_tid = Some new_current⌝ →
+            G new_current (cons (Tau (k tt)) (delete new_current_tid tp)) Φ
+        ∨ G (k tt) tp Φ
+        )) -∗
+      G (Vis (inl1 EYield) k) tp Φ
+    ) -∗
+    (□ ∀ Φ k tp,
+      (|={∅}=> G (k CurrentThread) (cons (k NewThread) tp) Φ) -∗
+      G (Vis (inl1 EFork) k) tp Φ
+    ) -∗
+    (□ ∀ Φ A (e : E A) k tp,
+      (|={∅}=> H _ e (λ a, G (k a) tp Φ) (λ a, |={⊤, ∅}=> G (k a) tp (λ _, False))) -∗
+      G (Vis (inr1 e) k) tp Φ
+    ) -∗
+    ∀ t tp Φ, wptp H t tp Φ -∗ G t tp Φ.
+  Proof.
+    iIntros "%Hne #HRet #HTau #HKillThread #HYield #HFork #HVis". iApply (wptp_iter G). iModIntro.
+    iIntros (t tp). destruct (itree_match t) as [[r ->]|[[t' ->]|[A [e [k ->]]]]].
+    - iIntros (Φ) "HΦ". iApply "HRet". rewrite /wptpF /=. by iMod "HΦ".
+    - iIntros (Φ) "Hwp". iApply "HTau". rewrite /wptpF //.
+    - iIntros (Φ) "Hwp". destruct e as [e|e]; rewrite /wptpF /=.
+      * destruct e.
+        + by iApply "HFork".
+        + iApply "HYield". by iMod "Hwp".
+        + iApply "HKillThread". iMod "Hwp". iMod "Hwp". iModIntro. iMod "Hwp". iModIntro.
+          iIntros (new_current_tid new_current Hidx). by iApply "Hwp".
+      * by iApply "HVis".
+  Qed.
+
+  Lemma wptp_inversion (t : itree (threadpoolE +' E) R) tp Φ G :
+    wptpF H G t tp Φ -∗
+    ( (∃ r, ⌜t ≅ Ret r⌝ ∧ (|={∅,⊤}=> Φ r))
+    ∨ (∃ t', ⌜t ≅ Tau t'⌝ ∧ |={∅}=> G t' tp Φ)
+    ∨ (∃ k, ⌜t ≅ Vis (inl1 EFork) k⌝ ∧
+      |={∅}=> G (k CurrentThread) (cons (k NewThread) tp) Φ
+      )
+    ∨ (∃ k, ⌜t ≅ Vis (inl1 EYield) k⌝ ∧ (
+      |={∅, ⊤}=> |={⊤, ∅}=>
+        (∀ new_current_tid new_current,
+            ⌜tp !! new_current_tid = Some new_current⌝ →
+            G new_current (cons (Tau (k tt)) (delete new_current_tid tp)) Φ
+        ∨ G (k tt) tp Φ
+        )
+      ))
+    ∨ (∃ k, ⌜t ≅ Vis (inl1 EKillThread) k⌝ ∧ (
+      |={∅, ⊤}=> |={⊤, ∅}=> ∀ new_current_tid new_current,
+        ⌜tp !! new_current_tid = Some new_current⌝ →
+        G new_current (delete new_current_tid tp) Φ
+      ))
+    ∨ (∃ A (e : E A) k, ⌜t ≅ Vis (inr1 e) k⌝ ∧
+      |={∅}=> H _ e (λ a, G (k a) tp Φ) (λ a, |={⊤, ∅}=> G (k a) tp (λ _, False))
+      )
+    ).
+  Proof.
+    iIntros "Hwptp".
+    destruct (itree_match t) as [[r ->]|[[t' ->]|[A [e [k ->]]]]].
+    - iLeft. iExists r. iSplit; first done. rewrite /wptpF /=. by iMod "Hwptp".
+    - iRight. iLeft. iExists t'. iSplit; first done. rewrite /wptpF /=. by iMod "Hwptp".
+    - destruct e as [e|e].
+      * destruct e.
+        + iRight. iRight. iLeft. iExists k. iSplit; first done. rewrite /wptpF /=. by iMod "Hwptp".
+        + iRight. iRight. iRight. iLeft. iExists k. iSplit; first done. rewrite /wptpF /=.
+          by iMod "Hwptp".
+        + iRight. iRight. iRight. iRight. iLeft. iExists k. iSplit; first done. rewrite /wptpF /=.
+          iMod "Hwptp". iMod "Hwptp". iModIntro. iMod "Hwptp". iModIntro.
+          iIntros (new_current_tid new_current Hidx). by iApply "Hwptp".
+      * iRight. iRight. iRight. iRight. iRight. iExists _, e, k. iSplit; first done.
+        rewrite /wptpF /= //.
+  Qed.
+End wptp_induction.
+
+Section wptp_proper.
+  Context {Σ : gFunctors} {R : Type} {E : Type → Type} `{!invGS_gen hlc Σ} {H : iHandler Σ E}.
+
+  (* TODO: Don't use instances for temporary class definitions. *)
+  Global Instance wptp_proper_unidirectional :
+    Proper (eqit (=) false false ==> Forall2 (eqit (=) false false) ==> (=) ==> (⊢)) (wptp (R:=R) H).
+  Proof.
+    iIntros (t1 t2 Ht tp1 tp2 Htp Φ Φ' <-).
+    epose (G := λ (t1 : leibnizO (itree (threadpoolE +' E) R)) (tp1 : leibnizO (list (itree (threadpoolE +' E) R))) (Φ : leibnizO R -d> iPropO Σ),
+      (∀ t2 tp2, ⌜t1 ≅ t2⌝ → ⌜Forall2 (eqit (=) false false) tp1 tp2⌝ → wptp H t2 tp2 Φ)%I).
+    iAssert (∀ t tp Φ, wptp H t tp Φ -∗ G t tp Φ)%I as "Hgen"; last first.
+    { iIntros "Hwptp". by iApply ("Hgen" with "Hwptp"). }
+    iApply (wptp_iter G); clear.
+    { intros n t1 t2 <- tp1 tp2 <- Φ1 Φ2 HΦ. rewrite /G. do 3 f_equiv.
+      do 3 f_equiv. rewrite /wptp. by apply least_fixpoint_ne.
+    }
+    iModIntro. iIntros (t1 tp1 Φ) "Hwptp". iIntros (t2 tp2 Ht Htp). rewrite wptp_unfold /wptpF.
+    punfold Ht. unfold eqit_ in Ht. remember (observe t1) as ot1. remember (observe t2) as ot2.
+    destruct Ht.
+    - by subst.
+    - rewrite /G. iMod "Hwptp". iModIntro. iApply "Hwptp". iPureIntro. pclearbot. apply REL. done.
+    - iMod "Hwptp". iModIntro. destruct e as [e|e].
+      * destruct e.
+        + simpl. rewrite /G. iApply "Hwptp". { iPureIntro. pclearbot. apply REL. }
+          iPureIntro. constructor; eauto. pclearbot. apply REL.
+        + simpl. iMod "Hwptp". iModIntro. iMod "Hwptp". iModIntro.
+          iIntros (new_current_tid new_current2 Hidx2).
+          apply Forall2_lookup_l with (P := eqit eq false false) (k := tp1) in Hidx2 as (new_current1&Hidx1&Hnew_current); last done.
+          iDestruct ("Hwptp" $! new_current_tid new_current1 Hidx1) as "[Hwptp|Hwptp]".
+          ++ iLeft. iApply "Hwptp"; first eauto. iPureIntro. constructor.
+             +++ f_equiv. f_equiv. pclearbot. apply REL.
+             +++ apply Forall2_delete. apply Htp.
+          ++ iRight. iApply "Hwptp"; last done. iPureIntro. pclearbot. apply REL.
+        + simpl. iMod "Hwptp". iModIntro. iMod "Hwptp". iModIntro.
+          iIntros (new_current_tid new_current2 Hidx2).
+          apply Forall2_lookup_l with (P := eqit eq false false) (k := tp1) in Hidx2 as (new_current1&Hidx1&Hnew_current); last done.
+          iApply ("Hwptp" $! new_current_tid new_current1 Hidx1); first done.
+          iPureIntro. apply Forall2_delete. apply Htp.
+      * iApply ihandler_mono; last done.
+        { iIntros (a) "Hwptp". iApply "Hwptp"; last done. pclearbot. iPureIntro. apply REL. }
+        iModIntro. iIntros (a) "Hwptp". iMod "Hwptp". iModIntro. iApply "Hwptp"; last done.
+        pclearbot. iPureIntro. apply REL.
+    - done.
+    - done.
+  Qed.
+  Global Instance wptp_proper :
+    Proper (eqit (=) false false ==> Forall2 (eqit (=) false false) ==> (=) ==> (⊣⊢)) (wptp (R:=R) H).
+  Proof.
+    intros t1 t2 Ht tp1 tp2 Htp Φ1 Φ2 HΦ.
+    iSplit.
+    - iIntros "Hwp". rewrite Ht Htp HΦ //.
+    - iIntros "Hwp". rewrite Ht Htp HΦ //.
+  Qed.
+End wptp_proper.
+
+Lemma big_sepL_delete' {Σ} A (Φ : A → iProp Σ) l i x :
+  l !! i = Some x →
+  ([∗ list] y ∈ l, Φ y) ⊣⊢
+  Φ x ∗ [∗ list] y ∈ (delete i l), Φ y.
+Proof.
+  intros Hidx. rewrite -(take_drop_middle l i x) // !big_sepL_app.
+  rewrite assoc -!(comm _ (Φ _)) -assoc -big_sepL_app. do 2 f_equiv.
+  rewrite -delete_take_drop. f_equiv. rewrite take_drop_middle //.
+Qed.
+
+Section threadpool_adequacy.
+  Context {Σ : gFunctors} {R : Type} {E : Type → Type} `{!invGS_gen hlc Σ}.
+  Context {H : iHandler Σ E}.
+
+  Lemma wp_wptp (t t' : itree (threadpoolE +' E) R) tp Φ :
+    WPi t' @ threadpoolH ⊕ H; ∅ {{ v, |={∅, ⊤}=> Φ v }} -∗
+    wptp H t tp Φ -∗
+    wptp H t (t' :: tp) Φ.
+  Proof.
+    epose (G := (λ (t : leibnizO (itree (threadpoolE +' E) R)) (tp : leibnizO (list (itree (threadpoolE +' E) R))) (Φ : leibnizO R -d> iPropO Σ),
+      wptp H t tp Φ ∧ ∀ t', WPi t' @ threadpoolH ⊕ H; ∅ {{ v, |={∅, ⊤}=> Φ v }} -∗ wptp H t (t' :: tp) Φ
+      )%I).
+    iAssert (∀ t tp Φ, wptp H t tp Φ -∗ G t tp Φ)%I as "Hgen"; last first.
+    { iIntros "Hwp Hwptp". iApply ("Hgen" with "Hwptp"); eauto. }
+    iApply (wptp_iter' (H := H) G); clear.
+    - intros n t1 t2 <- tp1 tp2 <- Φ1 Φ2 HΦ. rewrite /G.
+      apply bi.and_ne. { rewrite /wptp. by apply least_fixpoint_ne. } do 3 f_equiv.
+      * by do 3 f_equiv.
+      * apply least_fixpoint_ne; last done. reflexivity.
+    - iModIntro. iIntros (Φ tp r) "HΦ". iSplit; iIntros; rewrite wptp_unfold /wptpF //.
+    - iModIntro. iIntros (Φ tp t) "HG". iSplit.
+      { rewrite wptp_unfold /wptpF /=. iMod "HG". by iDestruct "HG" as "[Hwptp _]". }
+      iIntros (t') "Hwp". rewrite wptp_unfold /wptpF /=. iMod "HG". iDestruct "HG" as "[_ Hwptp]".
+      by iApply "Hwptp".
+    - iModIntro. iIntros (Φ tp k) "HG". iSplit.
+      { rewrite wptp_unfold /wptpF /=. iModIntro. iMod "HG". iModIntro. iMod "HG". iModIntro.
+        iIntros (new_current_tid new_current Hidx). by iDestruct ("HG" $! _ _ Hidx) as "[Hwptp _]".
+      }
+      iIntros (t') "Hwp". rewrite wptp_unfold /wptpF /=.
+      iModIntro. iMod "HG". iModIntro. iMod "HG". iModIntro.
+      iIntros (new_current_tid new_current Hidx).
+      destruct new_current_tid as [|new_current_tid']; first last.
+      * by iApply "HG".
+      * simpl. simpl in Hidx. injection Hidx as <-. rename t' into t.
+        unshelve epose (G' := (λne (t : leibnizO (itree (threadpoolE +' E) R)) (Φ_fupd : leibnizO R -d> iPropO Σ), ∀ Φ,
+          (∀ r, Φ_fupd r -∗ (|={∅, ⊤}=> Φ r)) -∗
+          (∀ new_current_tid new_current, ⌜tp !! new_current_tid = Some new_current⌝ → G new_current (delete new_current_tid tp) Φ) -∗
+           wptp H t tp Φ
+          )%I); try apply _; try solve_proper.
+        iAssert (∀ t Φ, WPi t @ threadpoolH ⊕ H; ∅ {{ Φ }} -∗ G' t Φ)%I as "Hgen"; last first.
+        { iApply ("Hgen" with "Hwp"); eauto. }
+        iApply (wpi_iter' (H := threadpoolH ⊕ H) G'); clear.
+        + intros n t1 t2 Ht tp1 tp2 <-. rewrite /G'. by do 2 f_equiv.
+        + iModIntro. iIntros (Φ r) "HΦ". rewrite /G' /=. iIntros (Φ') "Hfupd HG".
+          rewrite wptp_unfold /wptpF /=. by iApply "Hfupd".
+        + iModIntro. iIntros (Φ t) "HG'". rewrite /G' /=. iIntros (Φ') "Hfupd HG".
+          rewrite wptp_unfold /wptpF /=. iMod "HG'". iModIntro. by iApply ("HG'" with "Hfupd").
+        + iModIntro. iIntros (Φ A e k) "HH". rewrite /G' /=. iIntros (Φ') "Hfupd HG".
+          destruct e as [e|e]; first destruct e.
+          ++ rewrite wptp_unfold /wptpF /=. iMod "HH" as "[Hcurrent Hnew]". iApply "Hcurren"
+    iModIntro. iIntros (t tp Φ) "Hwptp".
+    iIntros (t') "Hwp".
+    iDestruct (wptp_inversion with "Hwptp") as "[(%r&->&HΦ)|[?|[?|[?|[?|?]]]]]".
+
+    unshelve epose (G' := (λne (t' : leibnizO (itree (threadpoolE +' E) R)) (Φ_fupd : leibnizO R -d> iPropO Σ),
+      ∀ Φ t tp, (∀ r, Φ_fupd r -∗ (|={∅, ⊤}=> Φ r)) -∗ wptpF H G t tp Φ -∗ wptp H t (t' :: tp) Φ
+      )%I); try apply _; try solve_proper.
+    iAssert (∀ t Φ_fupd, WPi t @ threadpoolH ⊕ H; ∅ {{ Φ_fupd }} -∗ G' t Φ_fupd)%I as "Hgen"; last first.
+    { iIntros (t') "Hwp". iApply ("Hgen" with "Hwp"); eauto. }
+    iApply (wpi_iter (H := threadpoolH ⊕ H) G'); first solve_proper.
+    clear. iModIntro. iIntros (t Φ) "Hwp". iIntros (Φ' t' tp) "Hwand Hwptp".
+    iDestruct (wptp_inversion with "Hwptp") as "[]".
+
+    unshelve epose (G := (λne (t' : leibnizO (itree (threadpoolE +' E) R)) (Φ_fupd : leibnizO R -d> iPropO Σ),
+      ∀ Φ t tp, (∀ r, Φ_fupd r -∗ (|={∅, ⊤}=> Φ r)) -∗ wptp H t tp Φ -∗ wptp H t (t' :: tp) Φ
+      )%I); try apply _; try solve_proper.
+    iAssert (∀ t Φ, WPi t @ threadpoolH ⊕ H; ∅ {{ Φ }} -∗ G t Φ)%I as "Hgen"; last first.
+    { iIntros "Hwp Hwptp". iApply ("Hgen" with "Hwp"); eauto. }
+    clear. iApply (wpi_iter (H := threadpoolH ⊕ H) G); first solve_proper.
+    iModIntro. iIntros (t' Φfupd) "Hwptp". iIntros (Φ t tp) "Hwand Hwp".
+    unshelve epose (G' := (λ (t : leibnizO (itree (threadpoolE +' E) R)) (tp : leibnizO (list (itree (threadpoolE +' E) R))) (Φ : leibnizO R -d> iPropO Σ),
+      ∀ t', wpiF (threadpoolH ⊕ H) (λ x : leibnizO (itree (threadpoolE +' E) R), G x) t' Φfupd -∗ wptp H t (t' :: tp) Φ
+      )%I).
+    iAssert (∀ t tp Φ, wptp H t tp Φ -∗ G' t tp Φ)%I as "Hgen"; last first.
+    { by iApply ("Hgen" with "Hwp"). }
+    iApply (wptp_iter' (H := H) G'); clear.
+    - intros n t1 t2 Ht tp1 tp2 <- Φ1 Φ2 HΦ. rewrite /G'. do 3 f_equiv.
+      apply least_fixpoint_ne; last done. reflexivity.
+    - iModIntro. iIntros (Φ tp r) "HΦ". rewrite /G'. iIntros (t') "Hwp".
+      rewrite wptp_unfold /wptpF. by iModIntro.
+    - iModIntro. iIntros (Φ tp t) "HG'". rewrite /G'. iIntros (t') "Hwp".
+      rewrite wptp_unfold /wptpF /=. iMod "HG'". iModIntro. by iApply "HG'".
+    - iModIntro. iIntros (Φ tp k) "HG'". rewrite /G'. iIntros (t') "Hwp".
+      rewrite wptp_unfold /wptpF /=. iModIntro. iIntros (new_current_tid new_current Hidx).
+      iApply "HG'".
+      iMod ("HG'" $! _ _ Hidx).
+    
+    clear. iIntros (t tp Φ) "Hwptp". iIntros (t') "Hwp".
+    iIntros (Φ t tp) "Hwand Hwptp". rewrite /G /=.
+      iEval (rewrite wptp_unfold /wptpF).
+
+  Lemma wp_wptp (t : itree (threadpoolE +' E) R) Φ :
+    WPi t @ (threadpoolH ⊕ H); ∅ {{ v, |={∅, ⊤}=> Φ v }} -∗
+    wptp H t [] Φ.
+  Proof.
+    unshelve epose (G := (λne (t : leibnizO (itree (threadpoolE +' E) R)) (Φ_fupd : leibnizO R -d> iPropO Σ),
+      ∀ Φ, (∀ r, Φ_fupd r -∗ (|={∅, ⊤}=> Φ r)) -∗ wptp H t [] Φ
+      )%I); try apply _; try solve_proper.
+    iAssert (∀ t Φ, WPi t @ threadpoolH ⊕ H; ∅ {{ Φ }} -∗ G t Φ)%I as "Hgen"; last first.
+    { iIntros "Hwp". iApply ("Hgen" with "Hwp"). eauto. }
+    iApply (wpi_iter' (H := threadpoolH ⊕ H) G); first solve_proper.
+    - clear. iModIntro. iIntros (Φfupd r) "HΦfupd". rewrite /G /=. iIntros (Φ) "Hwand".
+      rewrite wptp_unfold /wptpF /=. iMod "HΦfupd". iModIntro. by iApply "Hwand".
+    - clear. iModIntro. iIntros (Φfupd t) "Hwp". rewrite /G. simpl. iIntros (Φ) "Hwand".
+      rewrite wptp_unfold /wptpF /=. iMod "Hwp". iModIntro. iApply "Hwp".
+      iIntros (r) "HΦfupd". by iApply "Hwand".
+    - clear. iModIntro. iIntros (Φfupd t e k) "HH". iEval (rewrite /G /=). iIntros (Φ) "Hfupd".
+      destruct e as [e|e].
+      * rewrite wptp_unfold /wptpF /= /handle_threadpoolE /=.
+        destruct e.
+        + 
+    
   (** A technical version of adequacy, amenable to induction. See corollary below for a
   more meaningful statement. *)
   Theorem wpi_interleaving'
@@ -192,15 +596,38 @@ Section interleaving.
     WPi interleaving @ H; ∅ {{ r, |={∅, ⊤}=> Φ r }}.
   Proof.
     iIntros "%Hinter Htp Hcurrent".
+    unshelve epose (G := (λne (current : leibnizO (itree (threadpoolE +' E) R)) (Φ_fupd : leibnizO R -d> iPropO Σ),
+      ∀ interleaving tp Φ,
+        ⌜interleaves tp current interleaving⌝ →
+        (∀ r, Φ_fupd r -∗ (|={∅, ⊤}=> Φ r)) -∗
+        ([∗ list] thread ∈ tp, WPi thread @ threadpoolH ⊕ H; ⊤ {{ Φ }}) -∗
+        WPi interleaving @ H; ∅ {{ r, |={∅, ⊤}=> Φ r }}
+    )%I); try apply _; try solve_proper.
+    iAssert (∀ t Φ, WPi t @ threadpoolH ⊕ H; ∅ {{ Φ }} -∗ G t Φ)%I as "Hgen"; last first.
+    { iApply ("Hgen" with "Hcurrent [] [] Htp"); eauto. }
+    iApply (wpi_iter' (H := threadpoolH ⊕ H) G); first solve_proper.
+    - clear. iModIntro. iIntros (Φ r) "HΦ". iIntros (t tp Φfupd Hinter) "HΦfupd Htp".
+      punfold Hinter. inversion Hinter. subst. apply ret_observe_eqit in H3 as <-.
+      rewrite -wpi_ret'. by iApply "HΦfupd".
+    - clear. iModIntro. iIntros (Φ r) "HΦ". iIntros (t tp Φfupd Hinter) "HΦfupd Htp".
+      punfold Hinter. inversion Hinter. subst. apply tau_observe_eqit in H2 as <-.
+      rewrite -wpi_tau. iApply wpi_update. iMod "HΦ". pclearbot. by iApply ("HΦ" with "[] HΦfupd").
+    - clear -Sequential0. iModIntro.
+      iIntros (Φfupd A e k) "HH". iIntros (interleaving tp Φ Hinter) "HΦfupd Htp".
+      punfold Hinter.
+      inversion Hinter; simplify_K; simplify_eq.
+      * apply vis_observe_eqit in H5 as <-. rewrite -!wpi_vis'.
+        simpl. iMod "HH". iModIntro. iApply is_seq.
+        iApply (ihandler_mono with "[HΦfupd Htp] [] [HH //]").
+        + iIntros (a) "Hwp". iApply wpi_update_post. pclearbot. iApply ("Hwp" with "[] HΦfupd Htp").
+          iPureIntro. apply H2.
+        + iModIntro. by iIntros (t) "H".
+      * simplify_K. apply tau_observe_eqit in H5 as <-. rewrite -wpi_tau. simpl.
+        shelve.
+      * simplify_K. apply tau_observe_eqit in H5 as <-. simpl. rewrite -wpi_tau.
+
+
     iLöb as "IH" forall (tp current interleaving Hinter Φ). punfold Hinter.
-    inversion Hinter as
-      [tp' r Heqtp Heqcurrent Heqinterleaving
-      |current' tp' interleaving' Hinter' Heqtp Heqcurrent Heqinterleaving
-      |tp' A e k k' Hinter' Heqtp Heqcurrent Heqinterleaving
-      |tp' k new_current_tid new_current interleaving' Hidx Hinter' Heqtp Heqcurrent Heqinterleaving
-      |tp' k new_current_tid new_current interleaving' Hidx Hinter' Heqtp Heqcurrent Heqinterleaving
-      |tp' k interleaving' Hinter' Heqtp Heqcurrent Heqinterleaving
-      ].
     - (* Return tp' r *)
       apply ret_observe_eqit in Heqcurrent as <-. apply ret_observe_eqit in Heqinterleaving as <-.
       by rewrite -!wpi_ret'.
